try with set abstraction

Superposition_Calculus/Abstract_Substitution/Variable_Substitution.thy
@@ -6,13 +6,29 @@ locale set_spec =
   fixes
     contains :: "'x \<Rightarrow> 'set \<Rightarrow> bool"  and
     is_empty is_finite :: "'set \<Rightarrow> bool" and
-    subset_eq disjoint :: "'set \<Rightarrow> 'set \<Rightarrow> bool"
+    subset_eq disjoint :: "'set \<Rightarrow> 'set \<Rightarrow> bool" 
   assumes
     is_empty: "\<And>X. is_empty X \<longleftrightarrow> (\<forall>x. \<not> contains x X)" and
     is_finite: "\<And>X. is_finite X \<longleftrightarrow> (\<exists>n f. \<forall>x. contains x X \<longrightarrow> x \<in> f ` {i::nat. i < n})" and
     subset_eq: "\<And>X Y. subset_eq X Y \<longleftrightarrow> (\<forall>x. contains x X \<longrightarrow> contains x Y)" and
     disjoint: "\<And>X Y. disjoint X Y \<longleftrightarrow> 
-        (\<forall>x. contains x X \<longrightarrow> \<not> contains x Y) \<and> (\<forall>x. contains x Y \<longrightarrow> \<not> contains x X)" 
+        (\<forall>x. contains x X \<longrightarrow> \<not> contains x Y) \<and> (\<forall>x. contains x Y \<longrightarrow> \<not> contains x X)"
+
+(*locale set_spec' = 
+  fixes contains :: "'x \<Rightarrow> 'set \<Rightarrow> bool" 
+begin
+
+abbreviation "\<And>X. is_empty X \<equiv> \<forall>x. \<not> contains x X"
+
+abbreviation "\<And>X. is_finite X \<equiv> \<exists>n f. \<forall>x. contains x X \<longrightarrow> x \<in> f ` {i::nat. i < n}"
+
+abbreviation "\<And>X Y. subseteq X Y \<equiv> \<forall>x. contains x X \<longrightarrow> contains x Y"
+
+abbreviation "\<And>X Y. disjoint X Y \<equiv> 
+  (\<forall>x. contains x X \<longrightarrow> \<not> contains x Y) \<and> (\<forall>x. contains x Y \<longrightarrow> \<not> contains x X)"
+
+end*)
+
 
 interpretation set : set_spec where 
   contains = "(\<in>)" and is_empty = "\<lambda>X. X = {}" and is_finite = finite and subset_eq = "(\<subseteq>)" and
@@ -22,9 +38,63 @@ proof unfold_locales
     by (metis finite_conv_nat_seg_image rev_finite_subset subset_eq)
 qed auto
 
+(*interpretation set' : set_spec' where 
+  contains = "(\<in>)" 
+rewrites 
+  "set'.is_empty X \<equiv> Set.is_empty X" and
+  "set'.is_finite X = finite X" and
+  "set'.subseteq = (\<subseteq>)"and
+  "set'.disjoint X Y = (X \<inter> Y = {})"
+proof unfold_locales
+  show "(\<exists>n f. \<forall>x. x \<in> X \<longrightarrow> x \<in> f ` {i::nat. i < n}) = finite X"
+    by (metis finite_conv_nat_seg_image rev_finite_subset subset_eq)
+qed(auto simp: Set.is_empty_def)
+
+locale lifted_set_spec' = 
+  set_spec' contains + setset: set_spec' containsS
+  for contains :: "'x \<Rightarrow> 'set \<Rightarrow> bool" and containsS :: "'set \<Rightarrow> 'setset \<Rightarrow> bool" +
+  fixes Union :: "'setset \<Rightarrow> 'set"
+  assumes Union: "\<And>x X. contains x (Union X) \<longleftrightarrow> (\<exists>X'. containsS X' X \<and> contains x X')"
+begin
+
+lemma is_empty_Union: "is_empty (Union XX) \<longleftrightarrow> (\<forall>X. containsS X XX \<longrightarrow> is_empty X)"
+  by (meson Union)
+
+end
+
+interpretation set' : lifted_set_spec' where 
+  contains = "(\<in>)" and containsS = "(\<in>)" and Union = "\<Union>"
+   apply unfold_locales 
+  by auto*)
+
+locale lifted_set_spec = 
+  set_spec 
+  where contains = contains and is_empty = is_empty and is_finite = is_finite and 
+    subset_eq = subset_eq and disjoint = disjoint + 
+  setset: set_spec where contains = containsS and is_empty = is_emptyS and is_finite = is_finiteS and 
+    subset_eq = subset_eqS and disjoint = disjointS 
+  for contains :: "'x \<Rightarrow> 'set \<Rightarrow> bool" and containsS :: "'set \<Rightarrow> 'setset \<Rightarrow> bool" and 
+    is_empty is_finite subset_eq disjoint is_emptyS is_finiteS subset_eqS disjointS +
+  fixes Union :: "'setset \<Rightarrow> 'set" 
+  assumes Union: "\<And>x X. contains x (Union X) \<longleftrightarrow> (\<exists>X'. containsS X' X \<and> contains x X')"
+begin
+
+lemma is_empty_Union: "is_empty (Union XX) \<longleftrightarrow> (\<forall>X. containsS X XX \<longrightarrow> is_empty X)"
+  by (meson Union is_empty)
+  
+end 
+    
+
+interpretation set : lifted_set_spec where 
+  contains = "(\<in>)" and is_empty = "\<lambda>X. X = {}" and is_finite = finite and subset_eq = "(\<subseteq>)" and
+  disjoint = "\<lambda>X Y. X \<inter> Y = {}" and  containsS = "(\<in>)" and is_emptyS = "\<lambda>X. X = {}" and is_finiteS = finite and subset_eqS = "(\<subseteq>)" and
+  disjointS = "\<lambda>X Y. X \<inter> Y = {}" and Union = \<Union>
+proof unfold_locales
+qed auto
+
 interpretation fset : set_spec where 
   contains = "(|\<in>|)" and is_empty = "\<lambda>X. X = {||}" and is_finite = "\<lambda>_. True" and
-  subset_eq = "(|\<subseteq>|)" and disjoint = "\<lambda>X Y. X |\<inter>| Y = {||}"
+  subset_eq = "(|\<subseteq>|)" and disjoint = "\<lambda>X Y. X |\<inter>| Y = {||}" 
 proof unfold_locales
   show "\<And>X. True = (\<exists>n f. \<forall>x. x |\<in>| X \<longrightarrow> x \<in> f ` {i :: nat. i < n})"
     using finite_fset set.is_finite by blast
@@ -49,14 +119,12 @@ next
 qed
 
 locale variable_substitution = 
-  basic_substitution _ _ subst "\<lambda>a. is_empty (vars a)" +
-  set_spec where 
-  contains = contains and is_empty = is_empty  and is_finite = is_finite and 
-  subset_eq = subset_eq and disjoint = disjoint
+  set_spec contains +
+  basic_substitution _ _ subst "\<lambda>a. is_empty (vars a)" 
 for
   subst :: "'expression \<Rightarrow> ('variable \<Rightarrow> 'base_expression) \<Rightarrow> 'expression" (infixl "\<cdot>" 70) and
   vars :: "'expression \<Rightarrow> 'variables" and
-  contains is_empty is_finite subset_eq disjoint  +
+  contains :: "'variable \<Rightarrow> 'variables \<Rightarrow> bool" +
 assumes 
   subst_eq: "\<And>a \<sigma> \<tau>. (\<And>x. contains x (vars a) \<Longrightarrow> \<sigma> x = \<tau> x) \<Longrightarrow> a \<cdot> \<sigma> = a \<cdot> \<tau>"
 begin
@@ -78,8 +146,7 @@ lemma subst_reduntant_if [simp]:
 lemma subst_reduntant_if' [simp]: 
   assumes "disjoint (vars a) vars'"  
   shows "a \<cdot> (\<lambda>var. if contains var vars' then \<sigma>' var else \<sigma> var) = a \<cdot> \<sigma>"
-  using assms subst_eq subset_eq  disjoint
-  by fastforce
+  using assms subst_eq subset_eq disjoint by fastforce
 
 lemma subst_cannot_unground:
   assumes "\<not>is_ground (a \<cdot> \<sigma>)"  
@@ -155,14 +222,15 @@ lemma to_ground_inverse:
   assumes "is_ground f"
   shows "from_ground (to_ground f) = f"
   using assms 
-  by (metis f_inv_into_f from_ground_inverse mem_Collect_eq range_from_ground_iff_is_ground)
+  by (smt (verit, ccfv_threshold) from_ground_inverse grounding.range_from_ground_iff_is_ground grounding_axioms inj_onD inj_on_to_ground mem_Collect_eq rangeI)
 
 end
 
 (* TODO: base_variable_substitution *)
 locale variable_substitution_base = variable_substitution 
-  where subst = subst 
-  for subst :: "'expression \<Rightarrow> ('variable \<Rightarrow> 'expression) \<Rightarrow> 'expression"  (infixl "\<cdot>" 70) +
+  where subst = subst and contains = contains
+  for subst :: "'expression \<Rightarrow> ('variable \<Rightarrow> 'expression) \<Rightarrow> 'expression"  (infixl "\<cdot>" 70) and 
+    contains :: "'variable \<Rightarrow> 'variables \<Rightarrow> bool" +
   assumes 
     is_ground_iff:
       "\<And>exp. is_ground (exp \<cdot> \<gamma>) \<longleftrightarrow> (\<forall>x. contains x (vars exp) \<longrightarrow> is_ground (\<gamma> x))" and
@@ -229,7 +297,7 @@ locale variable_substitution_expansion = base: variable_substitution_base +
 for expanded_subst expanded_vars +
 assumes
   expanded_vars_vars: 
-    "(\<forall>x. is_empty (expanded_vars (expanded_subst x \<gamma>))) \<longleftrightarrow> (\<forall>x. is_empty (vars (x \<cdot> \<gamma>)))" and
+    "(\<forall>x. is_ground (expanded_subst x \<gamma>)) \<longleftrightarrow> (\<forall>x. base.is_ground (x \<cdot> \<gamma>))" and
   is_ground_iff:
   "is_ground (expanded_subst exp \<gamma>) \<longleftrightarrow> (\<forall>x. contains x (expanded_vars exp) \<longrightarrow> base.is_ground (\<gamma> x))"
 begin
@@ -265,34 +333,38 @@ lemma ground_exists: "\<exists>exp. is_ground exp"
 end
 
 locale variable_substitution_set = variable_substitution where 
-  contains = "(\<in>)" and is_empty = "\<lambda>X. X = {}" and is_finite = finite and subset_eq = "(\<subseteq>)" and
-  disjoint = "\<lambda>X Y. X \<inter> Y = {}"
+  contains = "(\<in>)" and is_empty = "\<lambda>X. X = {}" and is_finite = finite and
+  subset_eq = "(\<subseteq>)" and disjoint = "\<lambda>X Y. X \<inter> Y = {}"
 
 locale variable_substitution_base_set = variable_substitution_base where 
-  contains = "(\<in>)" and is_empty = "\<lambda>X. X = {}" and is_finite = finite and subset_eq = "(\<subseteq>)" and
-  disjoint = "\<lambda>X Y. X \<inter> Y = {}"
+  contains = "(\<in>)" and is_empty = "\<lambda>X. X = {}" and is_finite = finite and
+  subset_eq = "(\<subseteq>)" and disjoint = "\<lambda>X Y. X \<inter> Y = {}"
 
 (* TODO: With set spec *)
-locale variable_substitution_lifting_set = 
-  lifted: variable_substitution_set comp_subst id_subst base_subst base_vars
+locale variable_substitution_lifting = 
+  lifted: variable_substitution 
+  where comp_subst = comp_subst and id_subst = id_subst and subst = base_subst and 
+    vars = base_vars + 
+  lifted_set_spec where containsS = "(\<in>)"
   for 
     id_subst :: "'variable \<Rightarrow> 'base_expression" and
-    base_vars :: "'sub_expression \<Rightarrow> 'variable set" and
+    base_vars :: "'sub_expression \<Rightarrow> 'variables" and
+    containsS :: "'variables \<Rightarrow> 'variables set \<Rightarrow> bool" and
     comp_subst base_subst +
   fixes 
     map :: "('sub_expression \<Rightarrow> 'sub_expression) \<Rightarrow> 'expression \<Rightarrow> 'expression" and
-    to_set :: "'expression \<Rightarrow> 'sub_expression set" 
+    to_set :: "'expression \<Rightarrow> 'sub_expression set"
   assumes 
     map_comp: "\<And>d f g. map f (map g d) = map (f \<circ> g) d" and
     map_id: "map id d = d" and
     map_cong: "\<And>d f g. (\<And>c. c \<in> to_set d \<Longrightarrow> f c = g c) \<Longrightarrow> map f d = map g d" and
-    (* TODO: Better def? *)
+    (* TODO: name *)
     Union_range_to_set: "\<And>c. \<exists>d. c \<in> to_set d" and
-    to_set_map: "\<And>d f. to_set (map f d) = f ` to_set d"  
+    to_set_map: "\<And>d f. to_set (map f d) = f ` to_set d" 
 begin
 
-definition vars :: "'expression \<Rightarrow> 'variable set" where
-  "vars d \<equiv> \<Union>(base_vars ` to_set d)"
+definition vars :: "'expression \<Rightarrow> 'variables" where
+  "vars d \<equiv> Union (base_vars ` to_set d)"
 
 definition subst :: "'expression \<Rightarrow> ('variable \<Rightarrow> 'base_expression) \<Rightarrow> 'expression" where
   "subst d \<sigma> \<equiv> map (\<lambda>c. base_subst c \<sigma>) d"
@@ -315,7 +387,8 @@ lemma subst_in_to_set_subst:
   unfolding subst_def
   using to_set_map assms by auto
 
-sublocale variable_substitution_set comp_subst id_subst subst vars
+sublocale variable_substitution where
+  comp_subst = comp_subst and id_subst = id_subst and subst = subst and vars = vars and contains = contains 
 proof unfold_locales
   show "\<And>x a b. subst x (comp_subst a b) = subst (subst x a) b"
     using lifted.subst_comp_subst
@@ -326,21 +399,21 @@ next
     using map_id
     unfolding subst_def lifted.subst_id_subst id_def.
 next
-   show "\<And>d. vars d = {} \<Longrightarrow> \<forall>\<sigma>. subst d \<sigma> = d"
-     unfolding vars_def subst_def
-     using map_id_cong
-     by auto
+   show "\<And>x. is_empty (vars x) \<Longrightarrow> \<forall>\<sigma>. subst x \<sigma> = x"
+     unfolding vars_def subst_def is_empty_Union   
+     using map_id_cong 
+     by simp
 next
-  show "\<And>a \<sigma> \<tau>. (\<And>x. x \<in> vars a \<Longrightarrow> \<sigma> x = \<tau> x) \<Longrightarrow> subst a \<sigma> = subst a \<tau>"
+  show "\<And>a \<sigma> \<tau>. (\<And>x. contains x (vars a) \<Longrightarrow> \<sigma> x = \<tau> x) \<Longrightarrow> subst a \<sigma> = subst a \<tau> "
     unfolding vars_def subst_def
     using map_cong lifted.subst_eq
-    by (meson UN_I)
+    by (meson Union image_eqI)   
 qed
 
 (* TODO: name *)
 lemma is_ground_iff_base_is_ground: 
   "(\<forall>d. is_ground (subst d \<gamma>)) \<longleftrightarrow> (\<forall>c. lifted.is_ground (base_subst c \<gamma>))"
-proof(intro iffI allI)
+proof(rule iffI allI; rule allI)
   fix c 
   assume all_d_ground: "\<forall>d. is_ground (subst d \<gamma>)"
   show "lifted.is_ground (base_subst c \<gamma>)"
@@ -351,9 +424,9 @@ proof(intro iffI allI)
       using Union_range_to_set by auto
 
     then have "\<not>is_ground (subst d \<gamma>)"
-      using c_not_ground to_set_map
+      using c_not_ground to_set_map Union
       unfolding subst_def vars_def
-      by auto
+      using is_empty_Union by auto
 
     then show False
       using all_d_ground
@@ -366,7 +439,7 @@ next
   then show "is_ground (subst d \<gamma>)"
     unfolding vars_def subst_def
     using to_set_map
-    by auto 
+    using is_empty_Union by auto
 qed
 
 lemma is_ground_subst_iff_base_is_ground_subst [simp]: 
@@ -376,6 +449,11 @@ lemma is_ground_subst_iff_base_is_ground_subst [simp]:
   by presburger
 
 end
+
+locale variable_substitution_lifting_set = variable_substitution_lifting where 
+   contains = "(\<in>)" and is_empty = "\<lambda>X. X = {}" and is_finite = finite and
+  subset_eq = "(\<subseteq>)" and disjoint = "\<lambda>X Y. X \<inter> Y = {}" and containsS = "(\<in>)" and is_emptyS = "\<lambda>X. X = {}" and is_finiteS = finite and
+  subset_eqS = "(\<subseteq>)" and disjointS = "\<lambda>X Y. X \<inter> Y = {}" and Union = \<Union>
 
 locale based_variable_substitution_lifting_set = 
   variable_substitution_lifting_set where id_subst = id_subst and base_vars = base_vars and 
@@ -390,7 +468,8 @@ begin
 
 lemma is_ground_iff:
   "is_ground (subst exp \<gamma>) \<longleftrightarrow> (\<forall>x. x \<in> (vars exp) \<longrightarrow> base.is_ground (\<gamma> x))"
-  by (smt (verit) UNION_empty_conv(1) UN_iff UN_simps(10) lifted_is_ground_iff subst_def variable_substitution_lifting_set.to_set_map variable_substitution_lifting_set.vars_def variable_substitution_lifting_set_axioms)
+  using lifted_is_ground_iff subst_def to_set_map vars_def
+  by auto
 
 lemma obtain_ground_subst:
   obtains \<gamma> 
@@ -444,11 +523,11 @@ sublocale all_subst_ident_iff_ground
   where is_finite = finite and contains = "(\<in>)" and is_ground = is_ground and subst = subst 
 proof unfold_locales
   show "\<And>x. is_ground x = (\<forall>\<sigma>. subst x \<sigma> = x)"
-  proof(intro iffI allI)
-    show "\<And>x \<sigma>. is_ground x \<Longrightarrow> subst x \<sigma> = x"
+  proof(rule iffI allI)
+    show "\<And>x. is_ground x \<Longrightarrow> \<forall>\<sigma>. subst x \<sigma> = x"
       by simp
   next
-    fix d 
+    fix d x
     assume all_subst_ident: "\<forall>\<sigma>. subst d \<sigma> = d"
     
     show "is_ground d"
@@ -457,6 +536,7 @@ proof unfold_locales
 
       then obtain c where c_in_d: "c \<in> to_set d" and c_not_ground: "\<not>lifted.is_ground c"
         unfolding vars_def
+        using lifted.is_empty
         by blast
 
       then obtain \<sigma> where "base_subst c \<sigma> \<noteq> c" and "base_subst c \<sigma> \<notin> to_set d"
@@ -479,6 +559,7 @@ next
   obtain c where c_in_d: "c \<in> to_set d" and c_not_ground: "\<not>lifted.is_ground c"
     using d_not_ground
     unfolding vars_def
+    using lifted.is_empty
     by blast
 
   obtain \<sigma> where \<sigma>_not_ident: "base_subst c \<sigma> \<noteq> c" "base_subst c \<sigma> \<notin> \<Union> (to_set ` insert d ds)"
@@ -506,15 +587,15 @@ locale mylifting =
   all_subst_ident_iff_ground_lifting 
 
 locale variable_substitution_expansion_set = variable_substitution_expansion where 
-  contains = "(\<in>)" and is_empty = "\<lambda>X. X = {}" and is_finite = finite and subset_eq = "(\<subseteq>)" and
-  disjoint = "\<lambda>X Y. X \<inter> Y = {}" 
+  contains = "(\<in>)" and is_empty = "\<lambda>X. X = {}" and is_finite = finite and
+  subset_eq = "(\<subseteq>)" and disjoint = "\<lambda>X Y. X \<inter> Y = {}"
 
-locale variable_substitution_fset = variable_substitution where
+(*locale variable_substitution_fset = variable_substitution where
   contains = "(|\<in>|)" and is_empty = "\<lambda>X. X = {||}" and is_finite = "\<lambda>_. True" and
   subset_eq = "(|\<subseteq>|)" and disjoint = "\<lambda>X Y. X |\<inter>| Y = {||}"
 
 locale variable_substitution_expansion_fset = variable_substitution_expansion where 
   contains = "(|\<in>|)" and is_empty = "\<lambda>X. X = {||}" and is_finite = "\<lambda>_. True" and
-  subset_eq = "(|\<subseteq>|)" and disjoint = "\<lambda>X Y. X |\<inter>| Y = {||}"
+  subset_eq = "(|\<subseteq>|)" and disjoint = "\<lambda>X Y. X |\<inter>| Y = {||}"*)
 
 end
